code/ecdsap256/Hacl.P256.fsti
@@ -402,3 +402,24 @@ val is_more_than_zero_less_than_order: x: lbuffer uint8 (size 32) -> Stack bool
       r <==> (scalar > 0 && scalar < prime_p256_order)
     )
   )
+
+
+
+inline_for_extraction noextract
+val ecp256scalar_mult:
+    result:lbuffer uint8 (size 64)
+  -> pubKey:lbuffer uint8 (size 64)
+  -> scalar:lbuffer uint8 (size 32)
+  -> Stack bool
+    (requires fun h ->
+      live h result /\ live h pubKey /\ live h scalar /\
+      disjoint result pubKey /\ disjoint result scalar)
+    (ensures fun h0 r h1 ->
+      let pubKeyX = gsub pubKey (size 0) (size 32) in
+      let pubKeyY = gsub pubKey (size 32) (size 32) in
+      let pointX, pointY, flag =
+        ecp256_dh_r (as_seq h0 pubKeyX) (as_seq h0 pubKeyY) (as_seq h0 scalar) in
+      r == flag /\
+      modifies (loc result) h0 h1 /\
+      as_seq h1 (gsub result (size 0) (size 32)) == pointX /\
+      as_seq h1 (gsub result (size 32) (size 32)) == pointY)
